ArkLib.lean
@@ -38,11 +38,11 @@ import ArkLib.Data.UniPoly.Basic
 import ArkLib.Data.UniPoly.BasicOld
 import ArkLib.Data.UniPoly.PolynomialReflection
 import ArkLib.OracleReduction.Basic
-import ArkLib.OracleReduction.Composition.LiftContext
 import ArkLib.OracleReduction.Composition.Sequential.Basic
 import ArkLib.OracleReduction.Composition.Sequential.ProtocolSpec
 import ArkLib.OracleReduction.Equiv
 import ArkLib.OracleReduction.Execution
+import ArkLib.OracleReduction.LiftContext.Basic
 import ArkLib.OracleReduction.OracleInterface
 import ArkLib.OracleReduction.Prelude
 import ArkLib.OracleReduction.Security.Basic
