ArkLib/ProofSystem/Sumcheck/SingleRound.lean
@@ -6,7 +6,7 @@ Authors: Quang Dao
 
 import ArkLib.OracleReduction.Security.Basic
 import ArkLib.OracleReduction.Composition.Sequential.Basic
-import ArkLib.OracleReduction.Composition.LiftContext
+import ArkLib.OracleReduction.LiftContext.Basic
 import ArkLib.Data.Fin.Basic
 
 /-!
